kore/src/Syntax.v
@@ -10,78 +10,98 @@ Section Syntax.
 
   Context {Σ : Signature}.
 
-  Inductive Pattern :=
-  | kore_bevar (dbi : nat) (* (s : sort) ? *)
-  | kore_bsvar (dbi : nat) (* (s : sort) ? *)
-  | kore_fevar (x : evar) (* (s : sort) ? *)
-  | kore_fsvar (X : svar) (* (s : sort) ? *)
+  Inductive Pattern : list sort -> list sort -> sort -> Type :=
+  | kore_bevar {ex mu : list sort} {s : sort}
+               (idx : InTy s ex) : Pattern ex mu s
+  | kore_bsvar {ex mu : list sort} {s : sort}
+               (idx : InTy s mu) : Pattern ex mu s
+  | kore_fevar {ex mu : list sort} {s : sort}
+               (x : evar s) : Pattern ex mu s
+  | kore_fsvar {ex mu : list sort} {s : sort}
+               (X : svar s) : Pattern ex mu s
 
-  | kore_app   (σ : symbol) (* (ss : list sort) ? *) (args : list Pattern)
+  | kore_app   {ex mu : list sort} (* (ss : list sort) (explicit app arg sort)? *)
+               (σ : symbol)
+               (args : hlist (Pattern ex mu) (arg_sorts σ)) : Pattern ex mu (ret_sort σ)
 
-  | kore_bot   (s : sort)
-  | kore_top   (s : sort)
-  | kore_not   (φ : Pattern)     (* (s : sort) ? *)
-  | kore_and   (φ1 φ2 : Pattern) (* (s : sort) ? *)
-  | kore_or    (φ1 φ2 : Pattern) (* (s : sort) ? *)
-  | kore_imp   (φ1 φ2 : Pattern) (* (s : sort) ? *)
-  | kore_iff   (φ1 φ2 : Pattern) (* (s : sort) ? *)
+  | kore_bot   {ex mu : list sort}
+               (s : sort) : Pattern ex mu s
+  | kore_top   {ex mu : list sort}
+               (s : sort) : Pattern ex mu s
+  | kore_not   {ex mu : list sort} {s : sort}
+               (φ : Pattern ex mu s) : Pattern ex mu s
+  | kore_and   {ex mu : list sort} {s : sort}
+               (φ1 φ2 : Pattern ex mu s) : Pattern ex mu s
+  | kore_or    {ex mu : list sort} {s : sort}
+               (φ1 φ2 : Pattern ex mu s) : Pattern ex mu s
+  | kore_imp   {ex mu : list sort} {s : sort}
+               (φ1 φ2 : Pattern ex mu s) : Pattern ex mu s
+  | kore_iff   {ex mu : list sort} {s : sort}
+               (φ1 φ2 : Pattern ex mu s) : Pattern ex mu s
 
-  | kore_exists (s_var : sort) (φ : Pattern) (* (s_ret : sort) ? *)
-  | kore_forall (s_var : sort) (φ : Pattern) (* (s_ret : sort) ? *)
+  | kore_exists {ex mu : list sort} {s : sort}
+                (s_var : sort)
+                (φ : Pattern (s_var :: ex) mu s) : Pattern ex mu s
+  | kore_forall {ex mu : list sort} {s : sort}
+                (s_var : sort)
+                (φ : Pattern (s_var :: ex) mu s) : Pattern ex mu s
 
-  | kore_mu    (s_var : sort) (φ : Pattern)
-  | kore_nu    (s_var : sort) (φ : Pattern)
+  | kore_mu     {ex mu : list sort} {s : sort}
+                (φ : Pattern ex (s :: mu) s) : Pattern ex mu s
+  | kore_nu     {ex mu : list sort} {s : sort}
+                (φ : Pattern ex (s :: mu) s) : Pattern ex mu s
 
-  (* if s1 is omitted from the following constructs, well_sorted would
-     become not computable! *)
-  | kore_ceil  (s1 s2 : sort) (φ : Pattern)
-  | kore_floor (s1 s2 : sort) (φ : Pattern)
-  | kore_equals (s1 s2 : sort) (φ1 φ2 : Pattern)
-  | kore_in    (s1 s2 : sort) (φ1 φ2 : Pattern)
+  | kore_ceil   {ex mu : list sort} {s1 : sort}
+                (s2 : sort)
+                (φ : Pattern ex mu s1) : Pattern ex mu s2
+  | kore_floor  {ex mu : list sort} {s1 : sort}
+                (s2 : sort)
+                (φ : Pattern ex mu s1) : Pattern ex mu s2
+  | kore_equals {ex mu : list sort} {s1 : sort}
+                (s2 : sort)
+                (φ1 φ2 : Pattern ex mu s1) : Pattern ex mu s2
+  | kore_in     {ex mu : list sort} {s1 : sort}
+                (s2 : sort)
+                (φ1 φ2 : Pattern ex mu s1) : Pattern ex mu s2
 
 (*   | kore_next     (* (s : sort) ? *) (φ : Pattern)
   | kore_rewrites (* (s : sort) ? *) (φ1 φ2 : Pattern)
   | kore_dv       (s : sort) (s : string) *).
 
-
-  Section pat_ind.
-
+  Section pat_rect.
     Variables
-      (P : Pattern -> Prop).
+      (P : forall {ex mu s}, Pattern ex mu s -> Type).
     Hypotheses
-      (P_bevar : forall dbi, P (kore_bevar dbi))
-      (P_fevar : forall x, P (kore_fevar x))
-      (P_bsvar : forall dbi, P (kore_bsvar dbi))
-      (P_fsvar : forall x, P (kore_fsvar x))
+      (P_bevar : forall {ex mu s} idx, @P ex mu s (kore_bevar idx))
+      (P_fevar : forall {ex mu s} x, @P ex mu s (kore_fevar x))
+      (P_bsvar : forall {ex mu s} idx, @P ex mu s (kore_bsvar idx))
+      (P_fsvar : forall {ex mu s} x, @P ex mu s (kore_fsvar x))
 
-      (P_app : forall σ args, Forall P args -> P (kore_app σ args))
+      (P_app : forall {ex mu} σ (args : hlist (Pattern ex mu) (arg_sorts σ)), hlist_rect True (fun s ss x xs pf => prod (P x) pf) args -> P (kore_app σ args))
 
-      (P_bot : forall s, P (kore_bot s))
-      (P_top : forall s, P (kore_top s))
-      (P_not : forall φ, P φ -> P (kore_not φ))
-      (P_and : forall φ, P φ -> forall ψ, P ψ -> P (kore_and φ ψ))
-      (P_or : forall φ, P φ -> forall ψ, P ψ -> P (kore_or φ ψ))
-      (P_imp : forall φ, P φ -> forall ψ, P ψ -> P (kore_imp φ ψ))
-      (P_iff : forall φ, P φ -> forall ψ, P ψ -> P (kore_iff φ ψ))
+      (P_bot : forall {ex mu s}, @P ex mu s (kore_bot s))
+      (P_top : forall {ex mu s}, @P ex mu s (kore_top s))
+      (P_not : forall {ex mu s} (φ : Pattern ex mu s), P φ -> P (kore_not φ))
+      (P_and : forall {ex mu s} (φ : Pattern ex mu s), P φ -> forall ψ, P ψ -> P (kore_and φ ψ))
+      (P_or : forall {ex mu s} (φ : Pattern ex mu s), P φ -> forall ψ, P ψ -> P (kore_or φ ψ))
+      (P_imp : forall {ex mu s} (φ : Pattern ex mu s), P φ -> forall ψ, P ψ -> P (kore_imp φ ψ))
+      (P_iff : forall {ex mu s} (φ : Pattern ex mu s), P φ -> forall ψ, P ψ -> P (kore_iff φ ψ))
 
-      (P_exists : forall s φ, P φ -> P (kore_exists s φ))
-      (P_forall : forall s φ, P φ -> P (kore_forall s φ))
-      (P_mu : forall s φ, P φ -> P (kore_mu s φ))
-      (P_nu : forall s φ, P φ -> P (kore_nu s φ))
+      (P_exists : forall {ex mu s} s_var φ, @P (s_var :: ex) mu s φ -> @P ex mu s (kore_exists s_var φ))
+      (P_forall : forall {ex mu s} s_var φ, @P (s_var :: ex) mu s φ -> @P ex mu s (kore_forall s_var φ))
+      (P_mu : forall {ex mu s} φ, @P ex (s :: mu) s φ -> @P ex mu s (kore_mu φ))
+      (P_nu : forall {ex mu s} φ, @P ex (s :: mu) s φ -> @P ex mu s (kore_nu φ))
 
-      (P_ceil : forall s1 s2 φ, P φ -> P (kore_ceil s1 s2 φ))
-      (P_floor : forall s1 s2 φ, P φ -> P (kore_floor s1 s2 φ))
-      (P_equal : forall s1 s2 φ, P φ -> forall ψ, P ψ -> P (kore_equals s1 s2 φ ψ))
-      (P_in : forall s1 s2 φ, P φ -> forall ψ, P ψ -> P (kore_in s1 s2 φ ψ))
+      (P_ceil : forall {ex mu s1} s2 φ, @P ex mu s1 φ -> P (kore_ceil s2 φ))
+      (P_floor : forall {ex mu s1} s2 φ, @P ex mu s1 φ -> P (kore_floor s2 φ))
+      (P_equal : forall {ex mu s1} s2 φ, @P ex mu s1 φ -> forall ψ, @P ex mu s1 ψ -> P (kore_equals s2 φ ψ))
+      (P_in : forall {ex mu s1} s2 φ, @P ex mu s1 φ -> forall ψ, @P ex mu s1 ψ -> P (kore_in s2 φ ψ)).
 
-(*       (P_next : forall φ, P φ -> P (kore_next φ))
-      (P_rewrites : forall φ, P φ -> forall ψ, P ψ -> P (kore_rewrites φ ψ))
-      (P_dv : forall s str, P (kore_dv s str)) *).
-
-    Definition Pat_ind (φ : Pattern) : P φ.
+    Definition Pat_rect {ex mu s} (φ : Pattern ex mu s) : P φ.
     Proof.
-      revert φ.
-      refine (fix Pat_ind φ :=
+      revert ex mu s φ.
+
+      refine (fix Pat_rect {ex mu s} (φ : Pattern ex mu s) :=
       match φ with
        | kore_bevar dbi => P_bevar dbi
        | kore_fevar x => P_fevar x
@@ -90,8 +110,75 @@ Section Syntax.
 
        | kore_app σ args => _
 
-       | kore_bot s => P_bot s
-       | kore_top s => P_top s
+       | kore_bot s => P_bot
+       | kore_top s => P_top
+       | kore_not φ => P_not _ (Pat_rect φ)
+       | kore_and φ1 φ2 => P_and _ (Pat_rect φ1) _ (Pat_rect φ2)
+       | kore_or  φ1 φ2 => P_or _ (Pat_rect φ1) _ (Pat_rect φ2)
+       | kore_imp φ1 φ2 => P_imp _ (Pat_rect φ1) _ (Pat_rect φ2)
+       | kore_iff φ1 φ2 => P_iff _ (Pat_rect φ1) _ (Pat_rect φ2)
+
+       | kore_exists s φ => P_exists s _ (Pat_rect φ)
+       | kore_forall s φ => P_forall s _ (Pat_rect φ)
+
+       | kore_mu φ => P_mu _ (Pat_rect φ)
+       | kore_nu φ => P_nu _ (Pat_rect φ)
+
+       | kore_ceil s2 φ => P_ceil s2 _ (Pat_rect φ)
+       | kore_floor s2 φ => P_floor s2 _ (Pat_rect φ)
+       | kore_equals s2 φ1 φ2 => P_equal s2 _ (Pat_rect φ1) _ (Pat_rect φ2)
+       | kore_in    s2 φ1 φ2 => P_in s2 _ (Pat_rect φ1) _ (Pat_rect φ2)
+      end).
+      apply P_app.
+      induction args; simpl. 1: exact I.
+        split. 2: exact IHargs.
+        apply Pat_rect.
+    Defined.
+  End pat_rect.
+
+  Section pat_ind.
+    Variables
+      (P : forall {ex mu s}, Pattern ex mu s -> Prop).
+    Hypotheses
+      (P_bevar : forall {ex mu s} idx, @P ex mu s (kore_bevar idx))
+      (P_fevar : forall {ex mu s} x, @P ex mu s (kore_fevar x))
+      (P_bsvar : forall {ex mu s} idx, @P ex mu s (kore_bsvar idx))
+      (P_fsvar : forall {ex mu s} x, @P ex mu s (kore_fsvar x))
+
+      (P_app : forall {ex mu} σ (args : hlist (Pattern ex mu) (arg_sorts σ)), hlist_rect True (fun s ss x xs pf => (P x) /\ pf) args -> P (kore_app σ args))
+
+      (P_bot : forall {ex mu s}, @P ex mu s (kore_bot s))
+      (P_top : forall {ex mu s}, @P ex mu s (kore_top s))
+      (P_not : forall {ex mu s} (φ : Pattern ex mu s), P φ -> P (kore_not φ))
+      (P_and : forall {ex mu s} (φ : Pattern ex mu s), P φ -> forall ψ, P ψ -> P (kore_and φ ψ))
+      (P_or : forall {ex mu s} (φ : Pattern ex mu s), P φ -> forall ψ, P ψ -> P (kore_or φ ψ))
+      (P_imp : forall {ex mu s} (φ : Pattern ex mu s), P φ -> forall ψ, P ψ -> P (kore_imp φ ψ))
+      (P_iff : forall {ex mu s} (φ : Pattern ex mu s), P φ -> forall ψ, P ψ -> P (kore_iff φ ψ))
+
+      (P_exists : forall {ex mu s} s_var φ, @P (s_var :: ex) mu s φ -> @P ex mu s (kore_exists s_var φ))
+      (P_forall : forall {ex mu s} s_var φ, @P (s_var :: ex) mu s φ -> @P ex mu s (kore_forall s_var φ))
+      (P_mu : forall {ex mu s} φ, @P ex (s :: mu) s φ -> @P ex mu s (kore_mu φ))
+      (P_nu : forall {ex mu s} φ, @P ex (s :: mu) s φ -> @P ex mu s (kore_nu φ))
+
+      (P_ceil : forall {ex mu s1} s2 φ, @P ex mu s1 φ -> P (kore_ceil s2 φ))
+      (P_floor : forall {ex mu s1} s2 φ, @P ex mu s1 φ -> P (kore_floor s2 φ))
+      (P_equal : forall {ex mu s1} s2 φ, @P ex mu s1 φ -> forall ψ, @P ex mu s1 ψ -> P (kore_equals s2 φ ψ))
+      (P_in : forall {ex mu s1} s2 φ, @P ex mu s1 φ -> forall ψ, @P ex mu s1 ψ -> P (kore_in s2 φ ψ)).
+    Definition Pat_ind {ex mu s} (φ : Pattern ex mu s) : P φ.
+    Proof.
+      revert ex mu s φ.
+
+      refine (fix Pat_ind {ex mu s} (φ : Pattern ex mu s) :=
+      match φ with
+       | kore_bevar dbi => P_bevar dbi
+       | kore_fevar x => P_fevar x
+       | kore_bsvar dbi => P_bsvar dbi
+       | kore_fsvar x => P_fsvar x
+
+       | kore_app σ args => _
+
+       | kore_bot s => P_bot
+       | kore_top s => P_top
        | kore_not φ => P_not _ (Pat_ind φ)
        | kore_and φ1 φ2 => P_and _ (Pat_ind φ1) _ (Pat_ind φ2)
        | kore_or  φ1 φ2 => P_or _ (Pat_ind φ1) _ (Pat_ind φ2)
@@ -101,45 +188,40 @@ Section Syntax.
        | kore_exists s φ => P_exists s _ (Pat_ind φ)
        | kore_forall s φ => P_forall s _ (Pat_ind φ)
 
-       | kore_mu s φ => P_mu s _ (Pat_ind φ)
-       | kore_nu s φ => P_nu s _ (Pat_ind φ)
+       | kore_mu φ => P_mu _ (Pat_ind φ)
+       | kore_nu φ => P_nu _ (Pat_ind φ)
 
-       | kore_ceil s1 s2 φ => P_ceil s1 s2 _ (Pat_ind φ)
-       | kore_floor s1 s2 φ => P_floor s1 s2 _ (Pat_ind φ)
-       | kore_equals s1 s2 φ1 φ2 => P_equal s1 s2 _ (Pat_ind φ1) _ (Pat_ind φ2)
-       | kore_in    s1 s2 φ1 φ2 => P_in s1 s2 _ (Pat_ind φ1) _ (Pat_ind φ2)
-
-(*        | kore_next φ => P_next _ (Pat_ind φ)
-       | kore_rewrites φ ψ => P_rewrites _ (Pat_ind φ) _ (Pat_ind ψ)
-       | kore_dv s str => P_dv s str *)
+       | kore_ceil s2 φ => P_ceil s2 _ (Pat_ind φ)
+       | kore_floor s2 φ => P_floor s2 _ (Pat_ind φ)
+       | kore_equals s2 φ1 φ2 => P_equal s2 _ (Pat_ind φ1) _ (Pat_ind φ2)
+       | kore_in    s2 φ1 φ2 => P_in s2 _ (Pat_ind φ1) _ (Pat_ind φ2)
       end).
       apply P_app.
-      induction args; constructor.
-      by apply Pat_ind.
-      assumption.
+      induction args; simpl. 1: exact I.
+        split. 2: exact IHargs.
+        apply Pat_ind.
     Defined.
+
   End pat_ind.
 
-  Fixpoint pat_size (p : Pattern) : nat :=
+  Fixpoint pat_size {ex mu s} (p : Pattern ex mu s) : nat :=
   match p with
    | kore_imp φ1 φ2 | kore_iff φ1 φ2
    | kore_and φ1 φ2 | kore_or φ1 φ2
-   | kore_equals _ _ φ1 φ2 | kore_in _ _ φ1 φ2
+   | kore_equals _ φ1 φ2 | kore_in _ φ1 φ2
       => 1 + pat_size φ1 + pat_size φ2
    | kore_app σ args
-      => 1 + foldr (fun φ acc => pat_size φ + acc) 0 args
+      => 1 + hlist_rect 0 (λ _ _ a _ b, pat_size a + b) args
    | kore_exists _ φ | kore_forall _ φ
-   | kore_nu _ φ | kore_mu _ φ 
-   | kore_not φ | kore_ceil _ _ φ
-   | kore_floor _ _ φ
+   | kore_nu φ | kore_mu φ 
+   | kore_not φ | kore_ceil _ φ
+   | kore_floor _ φ
        => 1 + pat_size φ
    | kore_bevar _ | kore_fevar _
    | kore_bsvar _ | kore_fsvar _
    | kore_bot _ | kore_top _
        => 1
   end.
-
-
 End Syntax.
 
 Module Notations.
@@ -147,43 +229,43 @@ Module Notations.
   Declare Scope kore_scope.
   Delimit Scope kore_scope with kore.
 
-  Notation "'⊥(' s ')'" := (kore_bot s) (format "'⊥(' s ')'") : kore_scope.
-  Check ⊥( _ )%kore.
-  Notation "'Top(' s ')'" := (kore_top s) (format "'Top(' s ')'") : kore_scope.
-  Check Top( _ )%kore.
+  Notation "'⊥{' s '}'" := (kore_bot s) (format "'⊥{' s '}'") : kore_scope.
+  Check ⊥{ _ }%kore.
+  Notation "'Top{' s '}'" := (kore_top s) (format "'Top{' s '}'") : kore_scope.
+  Check Top{ _ }%kore.
   Notation "'!' p" := (kore_not p) (at level 71, format "'!'  p") : kore_scope.
-  Check (! ⊥(_))%kore.
+  Check (! ⊥{_})%kore.
   Notation "p1 'and' p2" := (kore_and p1 p2) (at level 72, format "p1  'and'  p2", left associativity) : kore_scope.
-  Check (⊥ and(_) Top)%kore.
+  Check (⊥{_} and Top{_})%kore.
   Notation "p1 'or' p2" := (kore_or p1 p2) (at level 73, format "p1  'or'  p2", left associativity) : kore_scope.
-  Check (⊥ or( _ ) Top)%kore.
+  Check (⊥{_} or Top{_})%kore.
   Notation "p1 '--->' p2" := (kore_imp p1 p2) (at level 75, format "p1  '--->'  p2", right associativity) : kore_scope.
-  Check (⊥ ---> Top(_))%kore.
+  Check (⊥{_} ---> Top{_})%kore.
   Notation "p1 '<--->' p2" := (kore_iff p1 p2) (at level 74, format "p1  '<--->'  p2") : kore_scope.
-  Check (⊥ <---> Top(_))%kore.
+  Check (⊥{_} <---> Top{_})%kore.
 
   Notation "s ⋅ pars" := (kore_app s pars) (at level 70, format "s  '⋅'  pars") : kore_scope.
-  Check (_ ⋅ [Top(_); Top(_)])%kore.
+  Fail Check (_ ⋅ [Top{_}; Top{_}]%hlist)%kore.
 
 
-  Notation "'ex' s1 ',' p" := (kore_exists s1 p) (at level 80, format "'ex'  s1 ','  p") : kore_scope.
-  Check (ex _ , ⊥(_))%kore.
-  Notation "'all' s1 ',' p" := (kore_forall s1 p) (at level 80, format "'all'  s1 ','  p") : kore_scope.
-  Check (all _ , ⊥(_))%kore.
+  Notation "∃ s1 ',' p" := (kore_exists s1 p) (at level 80, format "∃  s1 ','  p") : kore_scope.
+  Check (∃ _ , ⊥{_})%kore.
+  Notation "∀ s1 ',' p" := (kore_forall s1 p) (at level 80, format "∀  s1 ','  p") : kore_scope.
+  Check (∀ _ , ⊥{_})%kore.
 
-  Notation "'mu' s1 ',' p" := (kore_mu s1 p) (at level 80, format "'mu'  s1 ','  p") : kore_scope.
-  Check (mu _ , ⊥(_))%kore.
-  Notation "'nu' s1 ',' p" := (kore_nu s1 p) (at level 80, format "'nu'  s1 ','  p") : kore_scope.
-  Check (nu _ , ⊥(_))%kore.
+  Notation "μ ',' p" := (kore_mu p) (at level 80, format "μ ','  p") : kore_scope.
+  Check (μ , ⊥{_})%kore.
+  Notation "ν ',' p" := (kore_nu p) (at level 80, format "ν ','  p") : kore_scope.
+  Check (ν , ⊥{_})%kore.
 
-  Notation "'⌈(' s1 , s2 ')' p ⌉" := (kore_ceil s1 s2 p) (format "'⌈(' s1 ',' s2 ')'  p ⌉") : kore_scope.
-  Check (⌈(_, _) ⊥(_)⌉)%kore.
-  Notation "'⌊(' s1 , s2 ')' p ⌋" := (kore_floor s1 s2 p) (format "'⌊(' s1 ',' s2 ')'  p ⌋") : kore_scope.
-  Check ⌊(_, _) ⊥(_)⌋%kore.
-  Notation "p1 '=ml(' s1 ',' s2 ')' p2" := (kore_equals s1 s2 p1 p2) (at level 68, format "p1  '=ml(' s1 ',' s2 ')'  p2", left associativity) : kore_scope.
-  Check (⊥(_) =ml(_, _) Top(_))%kore.
-  Notation "p1 '⊆ml(' s1 ',' s2 ')' p2" := (kore_in s1 s2 p1 p2) (at level 68, format "p1  '⊆ml(' s1 ',' s2 ')'  p2", left associativity) : kore_scope.
-  Check (⊥(_) ⊆ml(_, _) Top(_))%kore.
+  Notation "'⌈{' s2 '}' p ⌉" := (kore_ceil s2 p) (format "'⌈{' s2 '}'  p ⌉") : kore_scope.
+  Check (⌈{_} ⊥{_}⌉)%kore.
+  Notation "'⌊{' s2 '}' p ⌋" := (kore_floor s2 p) (format "'⌊{' s2 '}'  p ⌋") : kore_scope.
+  Check ⌊{_} ⊥{_}⌋%kore.
+  Notation "p1 '=ml{' s2 '}' p2" := (kore_equals s2 p1 p2) (at level 68, format "p1  '=ml{' s2 '}'  p2", left associativity) : kore_scope.
+  Check (⊥{_} =ml{_} Top{_})%kore.
+  Notation "p1 '⊆ml{' s2 '}' p2" := (kore_in s2 p1 p2) (at level 68, format "p1  '⊆ml{' s2 '}'  p2", left associativity) : kore_scope.
+  Check (⊥{_} ⊆ml{_} Top{_})%kore.
 
 
 
@@ -226,6 +308,7 @@ Module Notations.
 
 End Notations.
 
+(*
 Section Sortedness.
   Import Notations.
   Context {Σ : Signature}.
@@ -340,7 +423,7 @@ Section Sortedness.
       well_sorted fe fs s φ ->
       well_sorted fe' fs' s φ.
   Proof.
-    induction φ using Pat_ind; intros * Hw1 Hw2 Hwf; try by constructor.
+    induction φ using Pat_rect; intros * Hw1 Hw2 Hwf; try by constructor.
     * simpl in *. destruct decide. 2: simpl in Hwf; congruence.
       clear Hwf. apply Hw1 in e.
       cbn. rewrite e. destruct decide; auto.
@@ -416,5 +499,5 @@ Section Sortedness.
       simpl. apply andb_split_1, andb_split_1 in Hwf. assumption.
   Defined.
 
-End Sortedness.
+End Sortedness. *)
 
