kore/src/Freshness.v
@@ -4,68 +4,61 @@ Section Freshness.
 
   Context {Σ : Signature}.
 
-  Fixpoint free_evars (φ : Pattern) {struct φ} : gset evar :=
+  Fixpoint free_evars {ex mu s}
+                      (φ : Pattern ex mu s)
+                      (sTarget : sort) {struct φ} : gset (evar sTarget) :=
   match φ with
-   | kore_fevar x => {[x]}
+   | @kore_fevar _ _ _ var_sort x =>
+       (* var_sort = s in this case *)
+       match decide (sTarget = var_sort) with
+       | left H => {[eq_rect_r evar x H]}
+       | right _ => ∅
+       end
    | kore_imp φ1 φ2 | kore_iff φ1 φ2
    | kore_and φ1 φ2 | kore_or φ1 φ2
-   | kore_equals _ _ φ1 φ2 | kore_in _ _ φ1 φ2
-      => free_evars φ1 ∪ free_evars φ2
+   | kore_equals _ φ1 φ2 | kore_in _ φ1 φ2
+      => free_evars φ1 sTarget ∪ free_evars φ2 sTarget
    | kore_app σ args
-      => foldr (fun x acc => free_evars x ∪ acc) ∅ args
+      => hlist_rect ∅ (fun _ _ x xs rest => free_evars x sTarget ∪ rest) args
    | kore_exists _ φ | kore_forall _ φ
-   | kore_mu _ φ | kore_nu _ φ 
-   | kore_not φ | kore_ceil _ _ φ | kore_floor _ _ φ
-      => free_evars φ
+   | kore_mu φ | kore_nu φ 
+   | kore_not φ | kore_ceil _ φ | kore_floor _ φ
+      => free_evars φ sTarget
    | kore_bevar _ | kore_fsvar _ | kore_bsvar _
    | kore_bot _ | kore_top _ => ∅
   end.
 
-  Fixpoint free_svars (φ : Pattern) {struct φ} : gset svar :=
+  Fixpoint free_svars {ex mu s}
+                      (φ : Pattern ex mu s)
+                      (sTarget : sort) {struct φ} : gset (svar sTarget) :=
   match φ with
-   | kore_fsvar X => {[X]}
+   | @kore_fsvar _ _ _ var_sort X =>
+       (* var_sort = s in this case *)
+       match decide (sTarget = var_sort) with
+       | left H => {[eq_rect_r svar X H]}
+       | right _ => ∅
+       end
    | kore_imp φ1 φ2 | kore_iff φ1 φ2
    | kore_and φ1 φ2 | kore_or φ1 φ2
-   | kore_equals _ _ φ1 φ2 | kore_in _ _ φ1 φ2
-      => free_svars φ1 ∪ free_svars φ2
+   | kore_equals _ φ1 φ2 | kore_in _ φ1 φ2
+      => free_svars φ1 sTarget ∪ free_svars φ2 sTarget
    | kore_app σ args
-      => foldr (fun x acc => free_svars x ∪ acc) ∅ args
+      => hlist_rect ∅ (fun _ _ x xs rest => free_svars x sTarget ∪ rest) args
    | kore_exists _ φ | kore_forall _ φ
-   | kore_mu _ φ | kore_nu _ φ 
-   | kore_not φ | kore_ceil _ _ φ | kore_floor _ _ φ
-      => free_svars φ
+   | kore_mu φ | kore_nu φ 
+   | kore_not φ | kore_ceil _ φ | kore_floor _ φ
+      => free_svars φ sTarget
    | kore_bevar _ | kore_fevar _ | kore_bsvar _
    | kore_bot _ | kore_top _ => ∅
   end.
 
-  Fixpoint dep_filter {A} (f : A -> bool) (l : list A) {struct l} :
-    list {a : A & f a} :=
-  match l with
-    | [] => []
-    | x::xs =>
-      (if f x as b0 return f x = b0 -> list {a : A & f a}
-      then fun P => existT x P :: dep_filter f xs
-      else fun P => dep_filter f xs
-      ) eq_refl
-  end.
-
-
-  Definition fresh_evar (s : sort) (φ : Pattern) : 
-    { x : evar & decide (evar_sort x = s) }.
-  Proof.
-    pose (elements (free_evars φ)) as fs.
-    pose (dep_filter (fun x => decide (evar_sort x = s)) fs) as filtered.
-    simpl in filtered.
-    exact (fresh filtered).
-  Defined.
-  Definition fresh_svar (s : sort) (φ : Pattern) :
-    { x : svar & decide (svar_sort x = s) }.
-  Proof.
-    pose (elements (free_svars φ)) as fs.
-    pose (dep_filter (fun x => decide (svar_sort x = s)) fs) as filtered.
-    simpl in filtered.
-    exact (fresh filtered).
-  Defined.
-
+  Definition fresh_evar {s} {ex mu}
+      (sTarget : sort) (φ : Pattern s ex mu) :
+      evar sTarget :=
+    fresh (elements (free_evars φ sTarget)).
+  Definition fresh_svar {s} {ex mu}
+      (sTarget : sort) (φ : Pattern s ex mu) :
+      svar sTarget :=
+    fresh (elements (free_svars φ sTarget)).
 
 End Freshness.
